Implementation/Lean/Cpn2mCrl2.lean
@@ -1,2 +1,6 @@
+import Cpn2mCrl2.Util
 import Cpn2mCrl2.Color
 import Cpn2mCrl2.Bag
+import Cpn2mCrl2.Expr
+import Cpn2mCrl2.Net
+import Cpn2mCrl2.Semantics
